Prove syneq_exp, syneq_defs, and syneq reflexive under certain conditions
Namely, when the code environment is FEMPTY, and the variable
equivalence maps are reflexive (or only reflexive).
This might be enough for the actual uses of reflexivity...

compiler/correctness/intLangScript.sml
@@ -158,14 +158,26 @@ val Cexp_only_ind =
 |> DISCH_ALL
 |> Q.GEN`P`
 
-The real reason why this doesn't work:
-  Expressions that go into an infinite loop via the code environment have no finite proof of equivalence to themselves.
-val syneq_exp_refl = store_thm("syneq_exp_refl",
-  ``(∀e c z V. (∀v. v < z ⇒ V v v) ⇒ syneq_exp c c z z V e e) ∧
-    (∀defs c z V U d1. (∀v. v < z ⇒ V v v) ∧ (∀v1 v2. U v1 v2 ⇒ v1 < LENGTH (d1++defs) ∧ (v2 = v1)) ∧ LENGTH d1 ≤ 1 ⇒ syneq_defs c c z z V (d1++defs) (d1++defs) U) ∧
-    (∀d c z V U. (∀v. v < z ⇒ V v v) ∧ (∀v1 v2. U v1 v2 ⇒ v1 < 1 ∧ (v2 = v1)) ⇒ syneq_defs c c z z V [d] [d] U) ∧
-    (∀x:num#Cexp. foo x) ∧
-    (∀es c z V. (∀v. v < z ⇒ V v v) ⇒ EVERY2 (syneq_exp c c z z V) es es)``,
+(*
+val lR_def = Define`lR c l2 l1 = l1 ∈ FDOM c ∧ l2 ∈ free_labs (c ' l1).body`
+val wfc_def = Define`wfc c = WF (lR c)`
+val wfc_FEMPTY = store_thm("wfc_FEMPTY",
+  ``wfc FEMPTY``,
+  rw[wfc_def] >>
+  qsuff_tac`lR FEMPTY = REMPTY`>-rw[WF_EMPTY_REL] >>
+  simp[FUN_EQ_THM,lR_def])
+*)
+
+val syneq_exp_FEMPTY_refl = store_thm("syneq_exp_FEMPTY_refl",
+  ``(∀e z V. (∀v. v < z ⇒ V v v) ⇒ syneq_exp FEMPTY FEMPTY z z V e e) ∧
+    (∀defs z V U d1. (∀v. v < z ⇒ V v v) ∧ (∀v1 v2. U v1 v2 = (v1 < LENGTH (d1++defs) ∧ (v2 = v1))) ∧
+      EVERY (λd. (∀az e. (d = INL (az,e)) ⇒ ∀z V. (∀v. v < z ⇒ V v v) ⇒ syneq_exp FEMPTY FEMPTY z z V e e)) d1 ⇒
+      syneq_defs FEMPTY FEMPTY z z V (d1++defs) (d1++defs) U) ∧
+    (∀d z V U. (∀v. v < z ⇒ V v v) ∧  (∀v1 v2. U v1 v2 = ((v1 = 0) ∧ (v2 = 0))) ⇒
+      (∀az e. (d = INL (az,e)) ⇒ ∀z V. (∀v. v < z ⇒ V v v) ⇒ syneq_exp FEMPTY FEMPTY z z V e e) ∧
+      syneq_defs FEMPTY FEMPTY z z V [d] [d] U) ∧
+    (∀(x:num#Cexp) z V. (∀v. v < z ⇒ V v v) ⇒ syneq_exp FEMPTY FEMPTY z z V (SND x) (SND x)) ∧
+    (∀es z V. (∀v. v < z ⇒ V v v) ⇒ EVERY2 (syneq_exp FEMPTY FEMPTY z z V) es es)``,
   ho_match_mp_tac (TypeBase.induction_of``:Cexp``) >>
   strip_tac >- (
     rw[Once syneq_exp_cases] >>
@@ -174,7 +186,7 @@ val syneq_exp_refl = store_thm("syneq_exp_refl",
   strip_tac >- rw[Once syneq_exp_cases] >>
   strip_tac >- (
     rw[] >> rw[Once syneq_exp_cases] >>
-    first_x_assum match_mp_tac >>
+    first_x_assum match_mp_tac >> simp[] >>
     Cases >> srw_tac[ARITH_ss][] ) >>
   strip_tac >- (
     rw[Once syneq_exp_cases] >>
@@ -187,12 +199,13 @@ val syneq_exp_refl = store_thm("syneq_exp_refl",
   strip_tac >- ( rw[] >> rw[Once syneq_exp_cases] ) >>
   strip_tac >- (
     rw[] >> rw[Once syneq_exp_cases] >>
-    first_x_assum match_mp_tac >>
+    first_x_assum match_mp_tac >> simp[] >>
     Cases >> srw_tac[ARITH_ss][] ) >>
   strip_tac >- (
     rw[] >> rw[Once syneq_exp_cases] >>
     qexists_tac`λv1 v2. v1 < LENGTH defs ∧ (v2 = v1)` >>
     conj_tac >- (
+      fsrw_tac[DNF_ss][] >>
       `defs = [] ++ defs` by rw[] >>
       POP_ASSUM SUBST1_TAC >>
       first_x_assum match_mp_tac >>
@@ -201,8 +214,10 @@ val syneq_exp_refl = store_thm("syneq_exp_refl",
     srw_tac[ARITH_ss][] >>
     Cases_on`v < LENGTH defs`>>fsrw_tac[ARITH_ss][]) >>
   strip_tac >- (
-    rw[] >> rw[Once syneq_exp_cases] >>
-    qexists_tac`λv1 v2. (v1,v2) = (0,0)` >> rw[]) >>
+    rw[] >>
+    simp_tac (srw_ss()) [Once syneq_exp_cases] >>
+    qexists_tac`λv1 v2. (v1,v2) = (0,0)` >>
+    rw[]) >>
   strip_tac >- (
     rw[] >> rw[Once syneq_exp_cases] >>
     fsrw_tac[DNF_ss][EVERY2_EVERY,EVERY_MEM,MEM_ZIP,MEM_EL]) >>
@@ -212,35 +227,64 @@ val syneq_exp_refl = store_thm("syneq_exp_refl",
   strip_tac >- ( rw[] >> rw[Once syneq_exp_cases] ) >>
   strip_tac >- (
     rw[] >>
-    Cases_on`d1`>>fs[] >- (
-      rw[Once syneq_exp_cases] ) >>
-    Cases_on`t`>>fsrw_tac[ARITH_ss][] >>
-    rw[Once syneq_exp_cases]
-    rw[] >> rw[Once syneq_exp_cases]
-    ) >>
+    simp[Once syneq_exp_cases] >>
+    rpt gen_tac >> strip_tac >>
+    res_tac >> fs[] >>
+    fs[EVERY_MEM,MEM_EL] >>
+    fsrw_tac[DNF_ss][] >>
+    Cases_on`EL n1 d1`>>fs[syneq_cb_aux_def,LET_THM,UNCURRY] >>
+    Cases_on`x`>>fs[syneq_cb_aux_def] >>
+    first_x_assum (match_mp_tac o MP_CANON) >>
+    qexists_tac`n1` >> simp[] >>
+    simp[syneq_cb_V_def] >>
+    srw_tac[ARITH_ss][] ) >>
   strip_tac >- (
     rw[] >>
+    fsrw_tac[DNF_ss][] >>
+    `d1 ++ d::defs = (d1 ++ [d]) ++ defs` by rw[] >>
+    pop_assum SUBST1_TAC >>
     first_x_assum match_mp_tac >>
-    simp[] >> metis_tac[] ) >>
+    simp[] >>
+    rw[] >>
+    first_x_assum (match_mp_tac o MP_CANON) >>
+    simp[] >>
+    qexists_tac`0`>>simp[] >>
+    qexists_tac`λv1 v2. (v1 = 0) ∧ (v2 = 0)` >> simp[] ) >>
   strip_tac >- (
-    rw[] >> ?????
+    rw[] >> fs[] >>
+    simp[Once syneq_exp_cases] >>
+    Cases_on`x`>>fs[syneq_cb_aux_def] >>
+    first_x_assum match_mp_tac >>
+    simp[syneq_cb_V_def] >>
+    srw_tac[ARITH_ss][] ) >>
   strip_tac >- (
-    rw[] >> ?????
-  strip_tac >- rw[] >>
+    rw[] >> fs[] >>
+    simp[Once syneq_exp_cases] >>
+    simp[syneq_cb_aux_def,UNCURRY] ) >>
+  strip_tac >- simp[] >>
   strip_tac >- rw[] >>
   strip_tac >- rw[])
 
-val syneq_refl = store_thm("syneq_refl",
-  ``∀v c. syneq c c v v``,
+val syneq_defs_FEMPTY_refl = store_thm("syneq_defs_FEMPTY_refl",
+  ``∀z V U defs. (∀v. v < z ⇒ V v v) ∧ (∀v1 v2. U v1 v2 = (v1 < LENGTH defs) ∧ (v2 = v1)) ⇒
+    syneq_defs FEMPTY FEMPTY z z V defs defs U``,
+  rw[] >>
+  `defs = [] ++ defs` by rw[] >>
+  pop_assum SUBST1_TAC >>
+  match_mp_tac (CONJUNCT1 (CONJUNCT2 syneq_exp_FEMPTY_refl)) >>
+  simp[])
+
+val syneq_FEMPTY_refl = store_thm("syneq_FEMPTY_refl",
+  ``∀v. syneq FEMPTY FEMPTY v v``,
   ho_match_mp_tac Cv_ind >> rw[] >>
   simp[Once syneq_cases] >>
   fsrw_tac[DNF_ss][EVERY_MEM,EVERY2_EVERY,FORALL_PROD,MEM_ZIP,MEM_EL] >>
   Cases_on`n < LENGTH defs`>>fsrw_tac[ARITH_ss][]>>
   map_every qexists_tac[`λv1 v2. v1 < LENGTH env ∧ (v2 = v1)`,`λv1 v2. v1 < LENGTH defs ∧ (v2 = v1)`] >>
   simp[] >>
-  match_mp_tac syneq_defs_refl >>
+  match_mp_tac syneq_defs_FEMPTY_refl >>
   simp[])
-val _ = export_rewrites["syneq_refl"]
+val _ = export_rewrites["syneq_FEMPTY_refl"]
 
 val inv_syneq_cb_V = store_thm("inv_syneq_cb_V",
   ``inv (syneq_cb_V az r1 r2 V V') = syneq_cb_V az r2 r1 (inv V) (inv V')``,
